WIP: repaired wrong spec of L2 in Serversepc.v

demo/Serverproof.v
@@ -24,16 +24,16 @@ Variable se tse: Genv.symtbl.
 Let ge := Genv.globalenv se b1.
 Let tge := Genv.globalenv tse b1.
 
-Definition wp := cajw_injp w.
-Definition sg := cajw_sg w.
-Definition rs0 := cajw_rs w.
-Definition m2 := match wp with injpw _ _ m2 _ => m2 end.
-Definition s2 := Mem.support m2.
+Let wp := cajw_injp w.
+Let sg := cajw_sg w.
+Let rs0 := cajw_rs w.
+Let m2 := match wp with injpw _ _ m2 _ => m2 end.
+Let s2 := Mem.support m2.
 Hypothesis GE: match_stbls injp wp se tse.
-Definition sp0 := rs0 RSP.
-Definition ra0 := rs0 RA.
-Definition vf0 := rs0 PC.
-Definition bx0 := rs0 RBX. (*only used callee_save register in this sample*)
+Let sp0 := rs0 RSP.
+Let ra0 := rs0 RA.
+Let vf0 := rs0 PC.
+Let bx0 := rs0 RBX. (*only used callee_save register in this sample*)
 
 Inductive new_blockv (s:sup) : val -> Prop :=
   new_blockv_intro : forall b ofs, ~ sup_In b s -> new_blockv s (Vptr b ofs).
@@ -411,7 +411,7 @@ Proof.
       assert (Val.inject f (Vptr b ofs) (Vptr b' (Ptrofs.add ofs (Ptrofs.repr delta)))).
       econstructor; eauto.
       eapply Genv.find_funct_transf in TRAN; eauto.
-    + rename m into m'. rename m1 into m. rename m3 into tm. rename m2' into tm'.
+    + rename m into m'. rename m1 into m. rename m2 into tm. rename m2' into tm'.
       econstructor; eauto.
       -- rewrite loc_arguments_int. cbn. rewrite H14.
          constructor; eauto.
@@ -431,11 +431,11 @@ Proof.
       intros r1 r2 s1' Hr Haf1.
       inv Haf1. inv Hr.
       cbn in *.
-      rename m into m1'. rename m3 into m2.
+      rename m into m1'.
       inv H36. rename m' into m1''. rename tm' into m2''.
       exists ((Mem.support m2), (State rs' m2'' true)). repeat apply conj.
       -- constructor. inversion H44; eauto.
-         unfold inner_sp. unfold s2. unfold CAinjp_b1.m2. cbn.
+         unfold inner_sp. cbn.
          rewrite H39. subst sp. rewrite H7.
          rewrite pred_dec_false; eauto.
       -- reflexivity.
@@ -471,7 +471,6 @@ Proof.
     intros. inv H; inv H0; inv H; cbn in *.
     ++ (*step_xor*)
       inv H14. symmetry in H7. inv H7.
-      rename m3 into m2.
       destruct (enter_fung_exec m2 rs0) as (m2'1 & m2'2 & m2'3 & m2'4 & sp &
                                               ALLOC & STORE1 & STORE2
                                              & LOAD1 & LOAD2 &  FREE & X & UNC); eauto.
@@ -566,11 +565,491 @@ Proof.
             repeat Pgso.
           + intros. cbn. repeat try Pgso; destruct r; cbn in *; try congruence; eauto.
             rewrite not_win in H. inv H.
-          + unfold s2. cbn. inversion X. eauto.
+          + cbn. inversion X. eauto.
       }
-      destruct H as [s2' [STEP MS]]. unfold s2. cbn.
+      destruct H as [s2' [STEP MS]].  cbn.
       exists (Mem.support m2, s2'). intuition eauto.
       revert STEP. generalize (Mem.support m2), (Genv.globalenv se1 b1); clear; intros.
+      pattern (State rs0 m2 true),E0,s2'. eapply plus_ind2; eauto; intros.
+    * apply plus_one; eauto.
+    * eapply plus_trans; eauto.
+      apply plus_one. auto.
+      ++ (*step_free*)
+     assert ({m2''1| Mem.free m2'' sb 0 16 = Some m2''1}).
+     {
+       apply Mem.range_perm_free; eauto.
+     }
+     destruct X as [m2'1 FREE'].
+     exploit Mem.free_right_inject. apply Hm''. eauto.
+     intros. exploit H11; eauto. intro INJ'.
+     symmetry in H3. inv H3.  inv H15.
+     assert (exists s2': Asm.state,
+             plus (Asm.step (Mem.support m2)) (Genv.globalenv se2 b1) (State rs m2'' true) E0 s2'
+             /\ ms (Return2 m) (Mem.support m2, s2')).
+     {
+       eexists. split.
+       econstructor. econstructor; eauto. find_instr.
+      (* Pfreeframe *)
+       simpl. cbn. unfold Mem.loadv. subst sp. rewrite H1 in *.
+       cbn in H12. cbn in H13. cbn. rewrite H12. rewrite H13.
+       Plia. cbn. rewrite FREE'. unfold nextinstr. cbn. rewrite H9.
+       cbn. compute_pc. reflexivity.
+       (*Pret*)
+       eapply star_step; eauto. econstructor; eauto. Simplif.
+       find_instr. cbn. unfold inner_sp. rewrite <- H.
+       rewrite pred_dec_true; eauto.
+       eapply star_refl. traceEq.
+      - constructor; eauto.
+        econstructor. instantiate (1:= INJ'). all: eauto.
+        + cbn. inv H8.
+          constructor; eauto.
+          -- eapply Mem.ro_unchanged_trans; eauto.
+             eapply Mem.ro_unchanged_free; eauto.
+          -- red. eauto using Mem.perm_free_3.
+          -- eapply mem_unchanged_on_trans_implies_valid. eauto.
+             instantiate (1 := fun b ofs => loc_out_of_reach f m1 b ofs /\ b <> sb).
+             eapply Mem.free_unchanged_on; eauto.
+             intros. intros [A B]. congruence.
+             intros. simpl. intuition auto. subst.
+             unfold Mem.valid_block in H8. cbn in H14. congruence.
+        + intros. cbn.
+          cbn. repeat try Pgso; eauto; destruct r; cbn in *; try congruence; eauto.
+        + cbn. cbn. inv H8.
+          erewrite (Mem.support_free _ _ _ _ _ FREE'). inv H26. eauto.
+      }
+      destruct H3 as [s2' [STEP MS]].  cbn.
+      exists (Mem.support m2, s2'). intuition eauto.
+      revert STEP. generalize (Mem.support m2), (Genv.globalenv se1 b1); clear; intros.
+      pattern (State rs m2'' true),E0,s2'. eapply plus_ind2; eauto; intros.
+      * apply plus_one; eauto.
+      * eapply plus_trans; eauto.
+        apply plus_one. auto.
+  - constructor. intros. inv H.
+Qed.
+
+End CAinjp_b1.
+
+Theorem self_simulation_wt :
+  forward_simulation wt_c wt_c L1 L1.
+Proof.
+  constructor. econstructor; eauto.
+  intros se1 se2 w Hse Hse1. cbn in *.
+  destruct w as [se' sg].
+  subst. inv Hse.
+  instantiate (1 := fun se1 se2 w _ => (fun s1 s2 => s1 = s2 /\ snd w = int_fptr__void_sg)). cbn beta. simpl.
+  instantiate (1 := state).
+  instantiate (1 := fun s1 s2 => False).
+  constructor; eauto.
+  - intros. simpl. inv H. reflexivity.
+  - intros. inv H. exists s1. exists s1. constructor; eauto. inv H0.
+    inv H1. cbn. eauto.
+  - intros. inv H. exists r1.
+    constructor; eauto.
+    constructor; eauto.
+    cbn. inv H0. constructor; eauto.
+  - intros. subst.
+    exists (se2, int__void_sg).
+    exists q1. inv H. repeat apply conj; simpl; auto.
+    + inv H0. constructor; cbn; eauto.
+    + constructor; eauto.
+    + intros. exists s1'. exists s1'. split; eauto.
+      inv H0. inv H1.
+      inv H. cbn. constructor; eauto.
+  - intros. inv H0. exists s1', s1'. split. left. econstructor; eauto.
+    econstructor. traceEq.
+    eauto.
+  - constructor. intros. inv H.
+Qed.
+
+(* Self-sim using ro *)
+Require Import ValueAnalysis.
+
+Section RO.
+
+Variable se : Genv.symtbl.
+Variable m0 : mem.
+
+Inductive sound_state : state -> Prop :=
+| sound_Callstateg : forall vf i m,
+    ro_acc m0 m -> sound_memory_ro se m ->
+    sound_state (Call1 vf i m)
+| sound_Callstatef : forall vf o m,
+    ro_acc m0 m -> sound_memory_ro se m ->
+    sound_state (Call2 vf o m)
+| sound_Returnstatef : forall m,
+    ro_acc m0 m -> sound_memory_ro se m ->
+    sound_state (Return1 m)
+| sound_Returnstateg : forall m,
+    ro_acc m0 m -> sound_memory_ro se m ->
+    sound_state (Return2 m).
+End RO.
+
+Definition ro_inv '(row se0 m0) := sound_state se0 m0.
+
+Lemma L1_ro : preserves L1 ro ro ro_inv.
+Proof.
+  intros [se0 m0] se1 Hse Hw. cbn in Hw. subst.
+  split; cbn in *.
+  - intros. inv H0; inv H.
+    + constructor; eauto.
+    + constructor; eauto.
+  - intros. inv H0. inv H. constructor; eauto.
+    constructor; eauto. red. eauto.
+  - intros. inv H0. inv H. simpl.
+    exists (row se1 m). split; eauto.
+    constructor; eauto. constructor; eauto.
+    intros r s' Hr AFTER. inv Hr. inv AFTER.
+    constructor. eapply ro_acc_trans; eauto.
+    eapply ro_acc_sound; eauto.
+  - intros. inv H0. inv H. constructor; eauto.
+Qed.
+
+Theorem self_simulation_ro :
+  forward_simulation ro ro L1 L1.
+Proof.
+  eapply preserves_fsim. eapply L1_ro; eauto.
+Qed.
+
+Lemma semantics_preservation_L1:
+  forward_simulation cc_compcert cc_compcert L1 (Asm.semantics b1).
+Proof.
+  unfold cc_compcert.
+  eapply compose_forward_simulations.
+  eapply self_simulation_ro.
+  eapply compose_forward_simulations.
+  eapply self_simulation_wt.
+  eapply compose_forward_simulations.
+  eapply CAinjp_simulation_L1.
+  eapply semantics_asm_rel; eauto.
+Qed.
+
+Section CAinjp_b2.
+
+Section MS.
+
+Variable w0: ccworld (ro @ cc_c_asm_injp).
+Let row := snd (fst w0).
+Let w := snd w0.
+Let wp:= cajw_injp w.
+
+Variable se tse: Genv.symtbl.
+
+Let ge := Genv.globalenv se b2.
+Let tge := Genv.globalenv tse b2.
+
+Hypothesis GE: match_stbls injp wp se tse.
+
+
+Let sg := cajw_sg w.
+Let rs0 := cajw_rs w.
+Let m2 := match wp with injpw _ _ m2 _ => m2 end.
+Let s2 := Mem.support m2.
+
+Let sp0 := rs0 RSP.
+Let ra0 := rs0 RA.
+Let vf0 := rs0 PC.
+Let bx0 := rs0 RBX. (*only used callee_save register in this sample*)
+
+Inductive match_state_ro_c_asm : state -> (sup * Asm.state) -> Prop :=
+|match_call1_ro m1 b b' ofs eb input j Hm delta:
+  wp = injpw j m1 m2 Hm ->
+  sp0 <> Vundef -> ra0 <> Vundef ->
+  Val.has_type sp0 Tptr -> Val.has_type ra0 Tptr ->
+  valid_blockv (Mem.support m2) sp0 ->
+  vf0 = Vptr eb Ptrofs.zero ->
+  Genv.find_funct_ptr tge eb = Some (Internal func_encrypt_b2) ->
+  j b = Some (b', delta) ->
+  rs0 RDI = Vint input ->
+  rs0 RSI = Vptr b' (Ptrofs.add ofs (Ptrofs.repr delta)) ->
+  sound_memory_ro se m1 ->
+  match_state_ro_c_asm (Call1 (Vptr b ofs) input m1) (s2, State rs0 m2 true)
+|match_call2_ro m1 b ofs j Hm (rs:regset) m1' m2' Hm' output sb b' delta eb:
+    let sp := rs RSP in let ra := rs RA in let vf := rs PC in
+    sp = Vptr sb Ptrofs.zero ->
+    wp = injpw j m1 m2 Hm ->
+    (forall ofs, loc_out_of_reach j m1 sb ofs) ->
+    Mem.range_perm m2' sb 0 16 Cur Freeable ->
+    injp_acc wp (injpw j m1' m2' Hm') ->
+    rs PC = Vptr b' (Ptrofs.add ofs (Ptrofs.repr delta)) ->
+    j b = Some (b', delta) -> rs RDI = Vint output ->
+    ra = Vptr eb (Ptrofs.repr 3) ->
+    Genv.find_funct_ptr tge eb = Some (Internal func_encrypt_b2) ->
+    sup_In sb (Mem.support m2') -> ~ sup_In sb s2 ->
+    (forall b d, j b = Some (sb,d) -> False) ->
+    vf <> Vundef ->
+    Mem.loadv Mptr m2' (Val.offset_ptr sp (Ptrofs.repr 8)) = Some ra0 ->
+    Mem.loadv Mptr m2' (Val.offset_ptr sp Ptrofs.zero) = Some sp0 ->
+    valid_blockv s2 sp0 ->
+     (forall r, is_callee_save r = true -> rs (preg_of r) = rs0 (preg_of r)) ->
+     Mem.sup_include s2 (Mem.support m2')  ->
+     sound_memory_ro se m1' ->
+     match_state_ro_c_asm (Call2 (Vptr b ofs) output m1') (s2, State rs m2' true)
+|match_return1_ro j j' m1 m1'' m2'' Hm Hm'' (rs:regset) eb sb:
+    let sp := rs RSP in
+    sp = Vptr sb Ptrofs.zero ->
+     wp = injpw j m1 m2 Hm ->
+     (forall ofs, loc_out_of_reach j m1 sb ofs) ->
+     Mem.range_perm m2'' sb 0 16 Cur Freeable ->
+     injp_acc wp (injpw j' m1'' m2'' Hm'') ->
+     rs PC = Vptr eb (Ptrofs.repr 3) ->
+     Genv.find_funct_ptr tge eb = Some (Internal func_encrypt_b2) ->
+     (forall b d, j' b = Some (sb,d) -> False) ->
+     Mem.loadv Mptr m2'' (Val.offset_ptr sp (Ptrofs.repr 8)) = Some ra0 ->
+     Mem.loadv Mptr m2'' (Val.offset_ptr sp Ptrofs.zero) = Some sp0 ->
+     ~ sup_In sb s2 ->
+     valid_blockv (Mem.support m2) sp0 ->
+     (forall r, is_callee_save r = true  -> rs (preg_of r) = rs0 (preg_of r)) ->
+     Mem.sup_include (Mem.support m2) (Mem.support m2'') ->
+     sound_memory_ro se m1'' ->
+     match_state_ro_c_asm (Return1 m1'') (s2, State rs m2'' true)
+|match_return2_ro j' m2'' m1'' (rs:regset) Hm'':
+  (injp_acc wp (injpw j' m1'' m2'' Hm'')) ->
+   rs RSP = rs0 RSP -> rs PC = rs0 RA ->
+   (forall r, is_callee_save r = true -> rs (preg_of r) = rs0 (preg_of r)) ->
+   Mem.sup_include s2 (Mem.support m2'') ->
+   sound_memory_ro se m1'' ->
+   match_state_ro_c_asm (Return2 m1'') (s2, State rs m2'' false).
+
+End MS.
+
+Ltac rlia := rewrite maxv; lia.
+Ltac Plia := try rewrite !Ptrofs.unsigned_zero; try rewrite!Ptrofs.unsigned_repr; try rlia.
+Ltac Ap64 := replace Archi.ptr64 with true by reflexivity.
+Ltac Ap64_in H0 := replace Archi.ptr64 with true in H0 by reflexivity.
+
+Lemma match_program_id' :
+  match_program (fun _ f0 tf => tf = id f0) eq b2 b2.
+Proof.
+  red. red. constructor; eauto.
+  constructor. constructor. eauto. simpl. econstructor; eauto.
+  constructor. eauto.
+  constructor; cbn; eauto. constructor; eauto.
+  econstructor.
+  apply linkorder_refl.
+  constructor. constructor; eauto.
+  constructor. eauto. econstructor.
+  apply linkorder_refl. eauto.
+  constructor; eauto.
+Qed.
+
+Ltac Pgso := rewrite Pregmap.gso; try congruence.
+Ltac Pgss := rewrite Pregmap.gss.
+
+Definition source_mem (w: injp_world) := match w with injpw _ m1 _ _ => m1 end.
+
+Lemma CAinjp_simulation_L2: forward_simulation
+                 (ro @ cc_c_asm_injp)
+                 (ro @ cc_c_asm_injp)
+                 L2 (Asm.semantics b2).
+Proof.
+  constructor. econstructor; eauto. instantiate (1 := fun _ _ _ => _). cbn beta.
+  intros se1 se2 w Hse Hse1. cbn in *. subst.
+  pose (ms := fun s1 s2 => match_state_ro_c_asm w se1 se2 s1 s2 /\
+                          cajw_sg (snd w) = int_fptr__void_sg /\
+                          ro_mem (snd (fst w)) = source_mem (cajw_injp (snd w))).
+  eapply forward_simulation_plus with (match_states := ms);
+  destruct w as  [[? [? ?]] [[f ? ? Hm] sg rs0]]; destruct Hse as [Hi Hse];
+    inv Hi; inv Hse; subst; cbn in *; eauto.
+  -  (*valid_query*)
+    intros q1' q2 [q1 [Hqi Hq]]. inv Hqi. inv Hq.
+    simpl. cbn in *.
+    generalize  match_program_id'. intro TRAN.
+    eapply Genv.is_internal_transf in TRAN; eauto.
+  - (* initial *)
+    intros q1' q2 s1 [q1 [Hqi Hq]] Hi1. inv Hi1.
+    inv Hqi. inv Hq.
+    inv H19. 2:{ rewrite size_int_fptr__void_sg_0 in H4. extlia. }
+    rename tm0 into m2. rename m into m1.
+    exists (Mem.support m2, State rs0 m2 true).
+    generalize  match_program_id'. intro TRAN.
+    eapply Genv.find_funct_transf in TRAN; eauto.
+    repeat apply conj.
+    + econstructor; eauto. inv H18.
+      subst tsp0. congruence.
+    + eauto.
+    + subst tvf. unfold Genv.find_funct in TRAN.
+      destruct (rs0 PC) eqn:HPC; try congruence. destruct Ptrofs.eq_dec; try congruence.
+      subst targs. rewrite loc_arguments_int_fptr in H12. simpl in H12. inv H12. inv H9.
+      inv H7. inv H8.
+      econstructor; cbn; eauto.
+      inv H18. subst tsp0. congruence.
+      inv H. eauto.
+    + eauto.
+    + inv H. eauto.
+  - (* final_state *)
+    intros s1 s2 r1 Hms Hf1. inv Hf1. inv Hms. inv H. cbn in *. inv H0.
+    exists (rs, m2''). split. constructor.
+    exists (cr Vundef m). split. constructor. constructor.
+    inv H3. constructor; eauto. inversion H18. eauto.
+    econstructor; eauto.
+    intros. inv H. rewrite size_int_fptr__void_sg_0 in H1. extlia.
+  - (* at_external*)
+    intros s1 s2 q1 MS EXT1. cbn. inv EXT1. inv MS.
+    inv H. cbn in *. inv H12. cbn in *.
+    symmetry in H9. inv H9.
+    eapply Genv.match_stbls_incr in H2; eauto.
+    2:{
+      intros. exploit H36; eauto. intros [A B].
+      unfold Mem.valid_block in *. split; eauto with mem.
+    }
+    exists ((s,row s m),(cajw (injpw f m m2' Hm'1) int__void_sg rs)).
+    exists (rs,m2'). repeat apply conj.
+    + econstructor; eauto.
+      generalize  match_program_id'. intro TRAN.
+      rewrite H13.
+      assert (Val.inject f (Vptr b ofs) (Vptr b' (Ptrofs.add ofs (Ptrofs.repr delta)))).
+      econstructor; eauto.
+      eapply Genv.find_funct_transf in TRAN; eauto.
+    + rename m into m'. rename m1 into m. rename m2 into tm. rename m2' into tm'.
+      exists (cq (Vptr b ofs) int__void_sg (Vint output :: nil) m'). split.
+      constructor. constructor. eauto.
+      econstructor; eauto.
+      -- rewrite loc_arguments_int. cbn. rewrite H15.
+         constructor; eauto.
+      -- rewrite H13. econstructor; eauto.
+      -- intros. rewrite size_int__void_sg_0 in H.
+         subst sp. rewrite H8 in H. inv H. extlia.
+      -- subst sp. rewrite H8. constructor.
+      -- subst ra. rewrite H16. constructor.
+      -- subst sp. rewrite H8. constructor. eauto.
+      -- eapply args_removed_tailcall_possible.
+         red. apply size_int__void_sg_0.
+      -- congruence.
+      -- subst ra. rewrite H16. congruence.
+    + constructor; eauto.
+    + constructor; eauto.
+      inversion H33. eauto with mem.
+    + (*after_external*)
+      intros r1' r2 s1' [r1 [Hri Hr]] Haf1.
+      inv Haf1. inv Hri. inv H. inv Hr.
+      cbn in *.
+      rename m into m1'. inv H0.
+      inv H39. rename m' into m1''. rename tm' into m2''.
+      exists ((Mem.support m2), (State rs' m2'' true)). repeat apply conj.
+      -- constructor. inversion H46; eauto.
+         unfold inner_sp.  cbn.
+         rewrite H42. subst sp. rewrite H8.
+         rewrite pred_dec_false; eauto.
+      -- reflexivity.
+      -- assert ( RANGEPERM: Mem.range_perm m2'' sb 0 16 Cur Freeable). 
+         { red. intros. inversion H46.
+           eapply unchanged_on_perm; eauto.
+           red. intros. exploit H20; eauto.
+         }
+         econstructor; cbn.
+         rewrite H42. eauto.
+         reflexivity. eauto. eauto. instantiate (1:= Hm'5). all: eauto.
+         ++ etransitivity. instantiate (1:= injpw f m1' m2' Hm'1).
+            constructor; eauto.
+            constructor; eauto.
+         ++ rewrite H43. eauto.
+         ++ intros. destruct (f b0) as [[sb' d']|] eqn: Hf.
+            * apply H47 in Hf as Hf'. rewrite H in Hf'. inv Hf'. eauto.
+            * exploit H48; eauto. intros [A B]. eauto.
+         ++ rewrite H42. subst sp. rewrite H8 in *. cbn in *.
+            eapply Mem.load_unchanged_on. apply H46. 2: eauto.
+            intros. red. intros. exploit H20; eauto.
+         ++ rewrite H42. subst sp. rewrite H8 in *. cbn in *.
+            eapply Mem.load_unchanged_on. apply H46. 2: eauto.
+            intros. red. intros. exploit H20; eauto.
+         ++ intros. rewrite H40; eauto.
+         ++ inversion H46. eauto with mem.
+         ++ eapply ro_acc_sound; eauto.
+     -- reflexivity.
+     -- reflexivity.            
+  - (*internal_steps*)
+    Local Opaque undef_regs.
+    Ltac compute_pc := rewrite Ptrofs.add_unsigned;
+                       rewrite Ptrofs.unsigned_one; rewrite Ptrofs.unsigned_repr; try rlia; cbn.
+    Ltac find_instr := cbn; try rewrite Ptrofs.unsigned_repr; try rlia; cbn; reflexivity.
+    intros. inv H; inv H0; inv H; cbn in *. inv H1.
+    ++ (*step_xor*)
+      inv H13. symmetry in H8. inv H8.
+      destruct (enter_fung_exec m2 rs0) as (m2'1 & m2'2 & m2'3 & m2'4 & sp &
+                                              ALLOC & STORE1 & STORE2
+                                             & LOAD1 & LOAD2 &  FREE & X & UNC); eauto.
+      apply Mem.fresh_block_alloc in ALLOC as FRESH.
+      exploit Mem.alloc_right_inject; eauto. intro INJ1.
+      exploit Mem.store_outside_inject; eauto.
+      intros. inversion Hm0. eauto. intro INJ2.
+      exploit Mem.store_outside_inject; eauto.
+      intros. inversion Hm0. eauto. intro INJ3.
+      exploit Mem.free_right_inject; eauto.
+      intros. inversion Hm0. eauto. intro INJ4.
+      rename H14 into Hpc. rename H18 into Hrdi. rename H19 into Hrsi.
+      set (key := Int.repr 42).
+      set (output := Int.xor input key).
+      assert (exists s2': Asm.state,
+             plus (Asm.step (Mem.support m2)) (Genv.globalenv se2 b2) (State rs0 m2 true) E0 s2'
+             /\ ms (Call2 (Vptr b ofs) output m1) (Mem.support m2, s2')).
+      { 
+        (*execution of Asm code*)
+        eexists. split.
+        - (*plus steps*)
+          econstructor.
+      (*Pallocframe*)
+      econstructor; eauto.
+      find_instr. simpl.
+      rewrite ALLOC. rewrite Ptrofs.add_zero. rewrite STORE1.
+      rewrite Ptrofs.add_zero_l. rewrite STORE2. unfold nextinstr.
+      repeat try Pgso. rewrite Hpc. cbn.
+      rewrite Ptrofs.add_zero_l. reflexivity.
+      (*xor*)
+      eapply star_step; eauto. econstructor; eauto. Simplif.
+      find_instr. simpl. Ap64. do 2 Pgso.
+      unfold nextinstr_nf, nextinstr. cbn.
+      rewrite undef_regs_pc. Pgso. Pgss. cbn.
+      rewrite Ptrofs.add_unsigned. rewrite Ptrofs.unsigned_one. simpl.
+      reflexivity.
+      (*call*)
+      eapply star_step; eauto. econstructor; eauto. Simplif. find_instr. cbn.
+      compute_pc. reflexivity.
+      apply star_refl. traceEq.
+        - constructor; eauto.
+          econstructor; eauto.
+          + do 3 Pgso. rewrite undef_regs_rsp.
+            Pgso. Pgso. 
+            Pgss. reflexivity.
+          + simpl. reflexivity.
+          + intros. red. intros. inversion Hm0. exploit mi_mappedblocks; eauto.
+          + apply Mem.free_range_perm in FREE. eauto.
+          + instantiate (1:= INJ3).
+          constructor; eauto.
+          -- red. eauto.
+          -- eapply Mem.ro_unchanged_trans.
+             eapply Mem.ro_unchanged_alloc; eauto.
+             eapply Mem.ro_unchanged_trans.
+             eapply Mem.ro_unchanged_store; eauto.
+             eapply Mem.ro_unchanged_store; eauto.
+             erewrite <- Mem.support_store; eauto.
+             red. eauto using Mem.perm_store_2.
+             red. intro. eapply Mem.valid_block_alloc; eauto.
+             red. intros. eapply Mem.perm_alloc_4; eauto.
+             intro. apply Mem.fresh_block_alloc in ALLOC.
+             subst. congruence.
+          -- red. intros.
+             inversion X. eapply unchanged_on_perm; eauto.
+          -- eauto with mem.
+          -- eapply Mem.unchanged_on_implies; eauto.
+             intros. cbn. eauto.
+          -- red. intros. congruence.
+          + repeat Pgso. rewrite undef_regs_rdi. Pgss.
+            unfold output. rewrite Hrdi. reflexivity.
+          + Pgso. Pgss. reflexivity.
+          + apply Mem.valid_new_block in ALLOC as VALID. unfold Mem.valid_block in *.
+          erewrite Mem.support_store. 2: eauto.
+          erewrite Mem.support_store; eauto.
+          + intros.
+            inversion Hm0. exploit mi_mappedblocks; eauto.
+          + Pgss. rewrite undef_regs_rsi. repeat Pgso.
+          + cbn. rewrite <- H. constructor; eauto.
+          + intros. cbn. repeat try Pgso; destruct r; cbn in *; try congruence; eauto.
+            rewrite not_win in H1. inv H1.
+          +  cbn. inversion X. eauto.
+      }
+      destruct H1 as [s2' [STEP MS]]. cbn.
+      exists (Mem.support m2, s2'). intuition eauto.
+      revert STEP. generalize (Mem.support m2), (Genv.globalenv se2 b2); clear; intros.
       pattern (State rs0 m2 true),E0,s2'. eapply plus_ind2; eauto; intros.
     * apply plus_one; eauto.
     * eapply plus_trans; eauto.
